ironfleet/src/Dafny/Distributed/Common/Framework/Timestamp.s.dfy
@@ -2,10 +2,13 @@ include "Environment.s.dfy"
 include "Host.s.dfy"
 include "DistributedSystem.s.dfy"
 include "../Collections/Seqs.i.dfy"
+include "../Collections/Maps2.s.dfy"
 
 abstract module Timestamp_s {
   import opened Collections__Seqs_i
   import opened DS_s : DistributedSystem_s
+  import opened Host_s
+  import opened Collections__Maps2_s
 
   type Timestamp = i : int | 0 <= i
 
